slabs bottom-up 18/n
apply starseq_upd2
remaining:
- rewriting f2 (Seq.index s2 n) as ~ emp
- proving aux lemmas
- applying starseq_unpack/pack
- fixing unification issue

src/SlabsUtils.fst
@@ -293,6 +293,222 @@ let t (md: array U64.t)
   )
   = ()
 
+
+//inline_for_extraction
+//let elim_intro_vdep_test_aux3
+//  (size_class: sc)
+//  (md: array U64.t{A.length md = 4})
+//  (md_as_seq1: G.erased (Seq.lseq U64.t 4))
+//  (md_as_seq2: G.erased (Seq.lseq U64.t 4))
+//  (arr: array U8.t{A.length arr = U32.v page_size})
+//  (pos: U32.t{U32.v pos < U32.v (nb_slots size_class)})
+//  : Lemma
+//  (requires
+//    Bitmap4.get
+//  )
+//  (
+//    (slab_vprop_aux_f size_class md_as_seq1 arr)
+//      (Seq.index
+//        (SeqUtils.init_u32_refined (U32.v (nb_slots size_class)))
+//        (U32.v pos)))
+//  (fun _ -> slot_vprop size_class arr pos)
+
+let a2bv = Bitmap4.array_to_bv2 #4
+
+inline_for_extraction
+let elim_intro_vdep_test_aux2_lemma
+  (size_class: sc)
+  (md: array U64.t{A.length md = 4})
+  (md_as_seq1: G.erased (Seq.lseq U64.t 4))
+  (md_as_seq2: G.erased (Seq.lseq U64.t 4))
+  (arr: array U8.t{A.length arr = U32.v page_size})
+  (pos: U32.t{U32.v pos < U32.v (nb_slots size_class)})
+  (k:nat{k <> (U32.v pos) /\ k < U32.v (nb_slots size_class)})
+  : Lemma
+  (requires (
+    let bm1 = a2bv (G.reveal md_as_seq1) in
+    let bm2 = a2bv (G.reveal md_as_seq2) in
+    Seq.index bm1 (Bitmap5.f #4 (U32.v pos)) = false /\
+    bm2 == Seq.upd bm1 (Bitmap5.f #4 (U32.v pos)) true
+  ))
+  (ensures
+    ((slab_vprop_aux_f size_class md_as_seq2 arr)
+      (Seq.index
+        (SeqUtils.init_u32_refined (U32.v (nb_slots size_class)))
+        k))
+    ==
+    ((slab_vprop_aux_f size_class md_as_seq1 arr)
+      (Seq.index
+        (SeqUtils.init_u32_refined (U32.v (nb_slots size_class)))
+        k))
+  )
+  =
+  //assert (U32.v (nb_slots size_class) <= 4 * U64.n);
+  //let k : k2:U32.t{U32.v k2 < 4 * U64.n}
+  //  = (U32.uint_to_t k) <: (k2:U32.t{U32.v k2 < 4 * U64.n}) in
+  //Bitmap4.get_lemma md_as_seq1 k;
+  //Bitmap4.get_lemma md_as_seq2 k;
+  //assert (Bitmap4.get md_as_seq1 k == Bitmap4.get md_as_seq2 k);
+  admit ()
+
+inline_for_extraction
+let elim_intro_vdep_test_aux2_lemma2
+  (size_class: sc)
+  (md: array U64.t{A.length md = 4})
+  (md_as_seq1: G.erased (Seq.lseq U64.t 4))
+  (md_as_seq2: G.erased (Seq.lseq U64.t 4))
+  (arr: array U8.t{A.length arr = U32.v page_size})
+  (pos: U32.t{U32.v pos < U32.v (nb_slots size_class)})
+  : Lemma
+  (requires (
+    let bm1 = a2bv (G.reveal md_as_seq1) in
+    let bm2 = a2bv (G.reveal md_as_seq2) in
+    Seq.index bm1 (Bitmap5.f #4 (U32.v pos)) = false /\
+    bm2 == Seq.upd bm1 (Bitmap5.f #4 (U32.v pos)) true
+  ))
+  (ensures
+    forall (k:nat{k <> (U32.v pos) /\ k < U32.v (nb_slots size_class)}).
+    ((slab_vprop_aux_f size_class md_as_seq2 arr)
+      (Seq.index
+        (SeqUtils.init_u32_refined (U32.v (nb_slots size_class)))
+        k))
+    ==
+    ((slab_vprop_aux_f size_class md_as_seq1 arr)
+      (Seq.index
+        (SeqUtils.init_u32_refined (U32.v (nb_slots size_class)))
+        k))
+  )
+  =
+  Classical.forall_intro (Classical.move_requires (
+    elim_intro_vdep_test_aux2_lemma
+      size_class md md_as_seq1 md_as_seq2 arr pos
+  ))
+
+let elim_intro_vdep_test_aux2_lemma3
+  (size_class: sc)
+  (md: array U64.t{A.length md = 4})
+  (md_as_seq1: G.erased (Seq.lseq U64.t 4))
+  (md_as_seq2: G.erased (Seq.lseq U64.t 4))
+  (arr: array U8.t{A.length arr = U32.v page_size})
+  (pos: U32.t{U32.v pos < U32.v (nb_slots size_class)})
+  : Lemma
+  (requires (
+    let bm1 = a2bv (G.reveal md_as_seq1) in
+    let bm2 = a2bv (G.reveal md_as_seq2) in
+    Seq.index bm1 (Bitmap5.f #4 (U32.v pos)) = false /\
+    bm2 == Seq.upd bm1 (Bitmap5.f #4 (U32.v pos)) true
+  ))
+  (ensures
+    ((slab_vprop_aux_f size_class md_as_seq2 arr)
+      (Seq.index
+        (SeqUtils.init_u32_refined (U32.v (nb_slots size_class)))
+        (U32.v pos)))
+    ==
+    none_as_emp #(Seq.seq U8.t)
+  )
+  = admit ()
+
+inline_for_extraction
+let elim_intro_vdep_test_aux2
+  (size_class: sc)
+  (md: array U64.t{A.length md = 4})
+  (md_as_seq1: G.erased (Seq.lseq U64.t 4))
+  (md_as_seq2: G.erased (Seq.lseq U64.t 4))
+  (arr: array U8.t{A.length arr = U32.v page_size})
+  (pos: U32.t{U32.v pos < U32.v (nb_slots size_class)})
+  : Steel unit
+  (
+  //A.varray md `star`
+  (
+    ((slab_vprop_aux_f size_class md_as_seq1 arr)
+      (Seq.index
+        (SeqUtils.init_u32_refined (U32.v (nb_slots size_class)))
+        (U32.v pos))) `star`
+  (
+  starseq
+    #(pos:U32.t{U32.v pos < U32.v (nb_slots size_class)})
+    #(option (Seq.seq U8.t))
+    (slab_vprop_aux_f size_class md_as_seq1 arr)
+    (slab_vprop_aux_f_lemma size_class md_as_seq1 arr)
+    (Seq.slice (SeqUtils.init_u32_refined (U32.v (nb_slots size_class))) 0 (U32.v pos))
+  `star`
+  starseq
+    #(pos:U32.t{U32.v pos < U32.v (nb_slots size_class)})
+    #(option (Seq.seq U8.t))
+    (slab_vprop_aux_f size_class md_as_seq1 arr)
+    (slab_vprop_aux_f_lemma size_class md_as_seq1 arr)
+    (Seq.slice (SeqUtils.init_u32_refined (U32.v (nb_slots size_class))) (U32.v pos + 1) (Seq.length (SeqUtils.init_u32_refined (U32.v (nb_slots size_class)))))
+  )))
+  (
+  fun _ ->
+  //A.varray md `star`
+  ((slab_vprop_aux_f size_class md_as_seq1 arr)
+      (Seq.index
+        (SeqUtils.init_u32_refined (U32.v (nb_slots size_class)))
+        (U32.v pos))) `star`
+  (
+    ((slab_vprop_aux_f size_class md_as_seq2 arr)
+      (Seq.index
+        (SeqUtils.init_u32_refined (U32.v (nb_slots size_class)))
+        (U32.v pos))) `star`
+  (
+  starseq
+    #(pos:U32.t{U32.v pos < U32.v (nb_slots size_class)})
+    #(option (Seq.seq U8.t))
+    (slab_vprop_aux_f size_class md_as_seq2 arr)
+    (slab_vprop_aux_f_lemma size_class md_as_seq2 arr)
+    (Seq.slice (SeqUtils.init_u32_refined (U32.v (nb_slots size_class))) 0 (U32.v pos))
+  `star`
+  starseq
+    #(pos:U32.t{U32.v pos < U32.v (nb_slots size_class)})
+    #(option (Seq.seq U8.t))
+    (slab_vprop_aux_f size_class md_as_seq2 arr)
+    (slab_vprop_aux_f_lemma size_class md_as_seq2 arr)
+    (Seq.slice (SeqUtils.init_u32_refined (U32.v (nb_slots size_class))) (U32.v pos + 1) (Seq.length (SeqUtils.init_u32_refined (U32.v (nb_slots size_class)))))
+  )))
+  (requires fun h0 ->
+    let bm1 = a2bv (G.reveal md_as_seq1) in
+    let bm2 = a2bv (G.reveal md_as_seq2) in
+    Seq.index bm1 (Bitmap5.f #4 (U32.v pos)) = false /\
+    bm2 == Seq.upd bm1 (Bitmap5.f #4 (U32.v pos)) true)
+  (ensures fun h0 _ h1 -> True)
+  =
+
+  elim_intro_vdep_test_aux2_lemma2
+    size_class md md_as_seq1 md_as_seq2 arr pos;
+  elim_intro_vdep_test_aux2_lemma3
+    size_class md md_as_seq1 md_as_seq2 arr pos;
+  starseq_upd2
+    #(pos:U32.t{U32.v pos < U32.v (nb_slots size_class)})
+    #(Seq.seq U8.t)
+    (slab_vprop_aux_f size_class md_as_seq1 arr)
+    (slab_vprop_aux_f size_class md_as_seq2 arr)
+    (slab_vprop_aux_f_lemma size_class md_as_seq1 arr)
+    (slab_vprop_aux_f_lemma size_class md_as_seq2 arr)
+    (SeqUtils.init_u32_refined (U32.v (nb_slots size_class)))
+    (SeqUtils.init_u32_refined (U32.v (nb_slots size_class)))
+    (U32.v pos)
+
+//  starseq_unpack_s
+//    #(pos:U32.t{U32.v pos < U32.v (nb_slots size_class)})
+//    #(option (Seq.seq U8.t))
+//    (slab_vprop_aux_f size_class md_as_seq arr)
+//    (slab_vprop_aux_f_lemma size_class md_as_seq arr)
+//    (SeqUtils.init_u32_refined (U32.v (nb_slots size_class)))
+//    (U32.v pos)
+
+
+    //let v0 = A.asel md h0 in
+    //let v1 = A.asel md h1 in
+    //let bm0 = Bitmap4.array_to_bv2 v0 in
+    //let bm1 = Bitmap4.array_to_bv2 v1 in
+    //let idx = Bitmap5.f #4 (U32.v pos) in
+    //Seq.index bm1 idx = true /\
+    //bm1 == Seq.upd bm0 idx true /\
+    //True)
+
+
+
 //#push-options "--z3rlimit 30"
 inline_for_extraction
 let elim_intro_vdep_test_aux
